Core/Ty/Structure.lean
@@ -17,21 +17,21 @@ namespace Core
 -- def SpineTy.to : SpineTy -> Ty
 -- | ⟨m , Ks, n, Ts, R⟩ => to' m Ks n Ts R
 
--- def Ty.spine : Ty -> Option (String × List Ty)
--- | gt#x => return (x, [])
--- | app f a => do
---   let (x, sp) <- spine f
---   (x, sp ++ [a])
--- | _ => none
+def Ty.spine : Ty -> Option (String × List Ty)
+| gt#x => return (x, [])
+| app f a => do
+  let (x, sp) <- spine f
+  (x, sp ++ [a])
+| _ => none
 
--- @[simp, grind =]
--- theorem Ty.spine_arrow {A B : Ty} : (A -:> B).spine = none := by simp [spine]
+@[simp, grind =]
+theorem Ty.spine_arrow {A B : Ty} : (A -:> B).spine = none := by simp [spine]
 
--- @[simp, grind =]
--- theorem Ty.spine_all : (∀[K] A).spine = none := by simp [spine]
+@[simp, grind =]
+theorem Ty.spine_all : (∀[K] A).spine = none := by simp [spine]
 
--- @[simp, grind =]
--- theorem Ty.spine_eq : (A ~[K]~ B).spine = none := by simp [spine]
+@[simp, grind =]
+theorem Ty.spine_eq : (A ~[K]~ B).spine = none := by simp [spine]
 
 -- def Ty.apply (t : Ty) : List Ty -> Ty
 -- | [] => t
